defined the monad FixM2, using just nat -> option A functions to represent potential non-termination

Monad.v
@@ -2,6 +2,8 @@
 Require Import Coq.Program.Tactics.
 Require Import Coq.Setoids.Setoid.
 Require Import Coq.Classes.Morphisms.
+Require Import Coq.Arith.Arith_base.
+
 
 (***
  *** The monad typeclass (unbundled approach)
@@ -13,26 +15,56 @@ Class MonadRet (M:Type -> Type) : Type :=
 Class MonadBind (M:Type -> Type) : Type :=
   bindM : forall {A B:Type}, M A -> (A -> M B) -> M B.
 
-Class MonadEq (M:Type -> Type) : Type :=
-  eqM : forall {A:Type}, M A -> M A -> Prop.
+Class MonadOrder (M:Type -> Type) : Type :=
+  leqM : forall {A:Type}, M A -> M A -> Prop.
+
+Notation "m1 '<<<' m2" := (leqM m1 m2) (at level 80, no associativity).
+
+Definition eqM `{MonadOrder} {A} : M A -> M A -> Prop :=
+  fun m1 m2 => m1 <<< m2 /\ m2 <<< m1.
 
 Notation "m1 '==' m2" := (eqM m1 m2) (at level 80, no associativity).
 
+Instance equiv_leqM_equiv_eqM `{MonadOrder} A {E:Equivalence (leqM (A:=A))} : Equivalence (eqM (A:=A)).
+  unfold eqM; constructor.
+  intro m; split; reflexivity.
+  intros m1 m2 H0; destruct H0; split; assumption.
+  intros m1 m2 m3 H1 H2; destruct H1; destruct H2;
+    split; transitivity m2; assumption.
+Qed.
+
 Class Monad M {MonadRet:MonadRet M} {MonadBind:MonadBind M}
-      {MonadEq:MonadEq M} : Prop :=
+      {MonadOrder:MonadOrder M} : Prop :=
   {
     monad_return_bind :
       forall A B x (f:A -> M B), bindM (returnM x) f == f x;
     monad_bind_return : forall A (m:M A), bindM m returnM == m;
     monad_assoc : forall A B C (m:M A) (f: A -> M B) (g: B -> M C),
                     bindM m (fun x => bindM (f x) g) == bindM (bindM m f) g;
-    monad_eq_equivalence :> forall A, Equivalence (eqM (A:=A));
-    monad_proper_return : forall A, Proper (@eq A ==> eqM (A:=A)) returnM;
+    monad_leq_preorder :> forall A, PreOrder (leqM (A:=A));
+    monad_proper_return : forall A, Proper (@eq A ==> leqM (A:=A)) returnM;
     monad_proper_bind :
       forall A B,
-        Proper (eqM (A:=A) ==>
-                    respectful (@eq A) (eqM (A:=B)) ==> eqM (A:=B)) bindM
+        Proper (leqM (A:=A) ==>
+                     respectful (@eq A) (leqM (A:=B)) ==> leqM (A:=B)) bindM
   }.
+
+
+(***
+ *** Stuff Needed for Rewriting w.r.t. eqM and leqM
+ ***)
+
+Add Parametric Relation `{Monad} A : (M A) (leqM (A:=A))
+  reflexivity proved by PreOrder_Reflexive
+  transitivity proved by PreOrder_Transitive
+as leqM_morphism.
+
+Instance eqM_Equivalence `{Monad} A : Equivalence (eqM (A:=A)).
+  constructor.
+  intro m; split; reflexivity.
+  intros m1 m2 H1; destruct H1; split; assumption.
+  intros m1 m2 m3 H1 H2; destruct H1; destruct H2; split; transitivity m2; assumption.
+Qed.
 
 Add Parametric Relation `{Monad} A : (M A) (eqM (A:=A))
   reflexivity proved by Equivalence_Reflexive
@@ -40,21 +72,41 @@ Add Parametric Relation `{Monad} A : (M A) (eqM (A:=A))
   transitivity proved by Equivalence_Transitive
 as eqM_morphism.
 
+Instance proper_eqM_leqM `{Monad} A : Proper (eqM (A:=A) ==> eqM (A:=A) ==> iff) (leqM (A:=A)).
+  intros x1 y1 eq1 x2 y2 eq2; destruct eq1; destruct eq2; split; intro.
+  transitivity x1; [ assumption | ]; transitivity x2; assumption.
+  transitivity y1; [ assumption | ]; transitivity y2; assumption.
+Qed.
+
+Instance monad_proper_return_eqM `{Monad} A :
+  Proper (@eq A ==> eqM (A:=A)) returnM.
+  intros x y e. rewrite e. reflexivity.
+Qed.
+
+Instance monad_proper_bind_eqM `{Monad} A B :
+  Proper (eqM (A:=A) ==> respectful (@eq A) (eqM (A:=B)) ==> eqM (A:=B)) bindM.
+  intros m1 m2 eqm f1 f2 eqf. destruct eqm.
+  split; (apply monad_proper_bind; [ assumption | ]; intros x1 x2 e;
+          destruct (eqf x1 x2 e)).
+  assumption.
+  rewrite e; replace (f1 x2) with (f1 x1); [ assumption | rewrite e; reflexivity ].
+Qed.
+
 
 (***
  *** The Identity Monad
  ***)
 
 Definition Identity (X:Type) := X.
-Instance IdMonadRet : MonadRet Identity := fun A x => x.
-Instance IdMonadBind : MonadBind Identity := fun A B m f => f m.
-Instance IdMonadEq : MonadEq Identity := @eq.
+Instance IdMonad_returnM : MonadRet Identity := fun A x => x.
+Instance IdMonad_bindM : MonadBind Identity := fun A B m f => f m.
+Instance IdMonad_leqM : MonadOrder Identity := @eq.
 Instance IdMonad : Monad Identity.
   constructor; intros; try reflexivity.
-  auto with typeclass_instances.
-  intros x y e; assumption.
-  intros m1 m2 eqm f1 f2 eqf.
-  rewrite eqm; apply eqf; reflexivity.
+  split; auto with typeclass_instances.
+  intros x y e; rewrite e; reflexivity.
+  intros m1 m2 leqm f1 f2 leqf.
+  rewrite leqm. apply leqf. reflexivity.
 Qed.
 
 
@@ -70,24 +122,31 @@ Instance StateT_returnM {S} `{Monad} : MonadRet (StateT S M) :=
 Instance StateT_bindM {S} `{Monad} : MonadBind (StateT S M) :=
   fun A B m f =>
     fun s => bindM (m s) (fun (sx:S * A) => let (s',x) := sx in f x s').
-Instance StateT_eqM {S} `{Monad} : MonadEq (StateT S M) :=
-  fun {A} m1 m2 => forall s, eqM (m1 s) (m2 s).
+Instance StateT_leqM {S} `{Monad} : MonadOrder (StateT S M) :=
+  fun {A} m1 m2 => forall s, leqM (m1 s) (m2 s).
+
+(* Extensionality law for == on StateT *)
+Lemma StateT_eqM_ext {S} `{Monad} A (m1 m2: StateT S M A) :
+  (forall s, m1 s == m2 s) -> m1 == m2.
+  unfold eqM, leqM, StateT_leqM; intro e; split; intros;
+    destruct (e s); assumption.
+Qed.
 
 (* The Monad instance for StateT *)
 Instance StateT_Monad S `{Monad} : Monad (StateT S M).
   constructor;
-  unfold returnM, StateT_returnM, bindM, StateT_bindM, eqM, StateT_eqM; intros.
+    unfold returnM, StateT_returnM, bindM, StateT_bindM;
+    intros; try (apply StateT_eqM_ext); intros.
   rewrite monad_return_bind; reflexivity.
   transitivity (bindM (m s) returnM); [ | apply monad_bind_return ].
-  apply monad_proper_bind; [ reflexivity | ].
+  apply monad_proper_bind_eqM; [ reflexivity | ].
   intros sx sy e; rewrite e; destruct sy; reflexivity.
   rewrite <- monad_assoc.
-  apply monad_proper_bind; [ reflexivity | ].
+  apply monad_proper_bind_eqM; [ reflexivity | ].
   intros sx sy e; rewrite e; destruct sy; reflexivity.
-  split; intros m1 m2; intros.
+  split; intro; intros; intro; intros.
   reflexivity.
-  symmetry; apply H0.
-  transitivity (m2 s); [ apply H0 | apply H1 ].
+  transitivity (y s); [ apply H0 | apply H1 ].
   intros x y e s; rewrite e; reflexivity.
   intros m1 m2 em f1 f2 ef s.
   apply monad_proper_bind; [ apply em | ].
@@ -101,10 +160,10 @@ Class MonadGet (S:Type) (M:Type -> Type) : Type := getM : M S.
 Class MonadPut (S:Type) (M:Type -> Type) : Type := putM : S -> M unit.
 
 Class MonadState S M {MonadRet:MonadRet M} {MonadBind:MonadBind M}
-      {MonadEq:MonadEq M} {MonadGet:MonadGet S M} {MonadPut:MonadPut S M}
+      {MonadOrder:MonadOrder M} {MonadGet:MonadGet S M} {MonadPut:MonadPut S M}
 : Prop :=
   {
-    monad_state_monad : @Monad M MonadRet MonadBind MonadEq;
+    monad_state_monad : @Monad M MonadRet MonadBind MonadOrder;
     monad_state_get_get :
       forall A f,
         bindM getM (fun s => bindM getM (f s)) ==
@@ -115,7 +174,7 @@ Class MonadState S M {MonadRet:MonadRet M} {MonadBind:MonadBind M}
                 bindM (putM s) (fun _ => returnM s);
     monad_state_put_put :
       forall s1 s2, bindM (putM s1) (fun _ => putM s2) == putM s2;
-    monad_state_proper_put : Proper (eq ==> eqM) putM
+    monad_state_proper_put : Proper (eq ==> leqM) putM
   }.
 
 (* The MonadState instance for StateT *)
@@ -127,94 +186,426 @@ Instance StateT_putM {S} `{Monad} : MonadPut S (StateT S M) :=
 
 Instance StateT_MonadState S `{Monad} : MonadState S (StateT S M).
   constructor; intros; try apply StateT_Monad;
-    unfold returnM, StateT_returnM, bindM, StateT_bindM, eqM, StateT_eqM,
+    unfold returnM, StateT_returnM, bindM, StateT_bindM,
            getM, StateT_getM, putM, StateT_putM; intros;
-    try (repeat (rewrite monad_return_bind); reflexivity).
+    try (apply StateT_eqM_ext; intros;
+         repeat (rewrite monad_return_bind); reflexivity).
   intros s1 s2 e s; rewrite e; reflexivity.
 Qed.
 
 
 (***
- *** The Least Fixed-Point / Non-Termination Transformer
+ *** The Least Fixed-Point / Non-Termination Monad
  ***)
 
 (* The non-termination monad as sets with at most one element *)
-Definition NonTermM X : Type :=
+Definition FixM X : Type :=
   { S:X -> Prop | forall x y, S x /\ S y -> x = y }.
 
-Program Instance NonTermM_returnM : MonadRet NonTermM :=
+Program Instance FixM_returnM : MonadRet FixM :=
   fun A x => (fun y => x = y).
 
-Definition NonTermM_map {X Y} (m:NonTermM X) (f:X -> NonTermM Y) : Y -> Prop :=
+(* Helper for defining bind on FixM *)
+Definition FixM_map {X Y} (m:FixM X) (f:X -> FixM Y) : Y -> Prop :=
   fun y => exists x, proj1_sig m x /\ proj1_sig (f x) y.
 
-Definition NonTermM_map_proof {X Y} (m:NonTermM X) (f:X -> NonTermM Y) :
-  forall x y, NonTermM_map m f x /\ NonTermM_map m f y -> x = y.
-  unfold NonTermM_map; intros; repeat (destruct H); repeat (destruct H0).
+(* Helper for the helper for defining bind on FixM *)
+Definition FixM_map_proof {X Y} (m:FixM X) (f:X -> FixM Y) :
+  forall x y, FixM_map m f x /\ FixM_map m f y -> x = y.
+  unfold FixM_map; intros; repeat (destruct H); repeat (destruct H0).
   unfold proj1_sig in * |- *; destruct m.
   rewrite (e x1 x0 $(split; assumption)$) in H2.
   destruct (f x0).
   apply e0; split; assumption.
 Qed.
 
-Instance NonTermM_bindM : MonadBind NonTermM :=
+Instance FixM_bindM : MonadBind FixM :=
   fun (A B:Type) m f =>
-    exist _ (NonTermM_map m f) (NonTermM_map_proof m f).
+    exist _ (FixM_map m f) (FixM_map_proof m f).
 
-Instance NonTermM_eqM : MonadEq NonTermM :=
-  fun {A} m1 m2 => forall x, proj1_sig m1 x <-> proj1_sig m2 x.
+Instance FixM_leqM : MonadOrder FixM :=
+  fun {A} m1 m2 => forall x, proj1_sig m1 x -> proj1_sig m2 x.
 
-Instance NonTermM_Monad : Monad NonTermM.
-  constructor;
-    unfold returnM, NonTermM_returnM, bindM, NonTermM_bindM, eqM, NonTermM_eqM,
-           NonTermM_map, NonTermM_map, proj1_sig;
-    intros.
-  
-
-
-
-  replace f with (fun x => exist _ (proj1_sig (f x)) (proj2_sig (f x)));
-   [ | apply functional_extensionality; intros; destruct (f x0); reflexivity ].
-  apply eq_dep_eq_sig; apply eq_dep1_dep. eapply eq_dep1_intro.
-  Unshelve. Focus 4.
-  apply functional_extensionality; intros.
-
-  assert 
-
-
-  replace f with (fun x => exist _ (proj1_sig_and f x) (proj2_sig_and f x)).
-  generalize (proj2_sig_and f).
-
-
-  generalize (proj1_sig_and f).
-
-   [ | apply functional_extensionality; intros; destruct (f x0); reflexivity ].
-
-
-
-(* The empty Type01 *)
-Program Definition empty_Type01 X : Type01 X := (fun _ => False).
-Obligation 1.
-elimtype False; assumption.
+(* Extensionality law for <<< on FixM *)
+Lemma FixM_leqM_ext A (m1 m2: FixM A) :
+  (forall x, proj1_sig m1 x -> proj1_sig m2 x) -> m1 <<< m2.
+  intros H x; apply H.
 Qed.
 
-(* The singleton Type01 *)
-Program Definition singleton_Type01 {X} (x:X) : Type01 X := (fun y => x = y).
+(* Extensionality law for == on FixM *)
+Lemma FixM_eqM_ext A (m1 m2: FixM A) :
+  (forall x, proj1_sig m1 x <-> proj1_sig m2 x) -> m1 == m2.
+  intro equiv; split; intros x elem; destruct (equiv x);
+    [ apply H | apply H0 ]; assumption.
+Qed.
 
-(* Mapping a Type01 *)
-Program Definition map_Type01 {X Y} (f: X -> Type01 )
+(* Monad instance for FixM *)
+Instance FixM_Monad : Monad FixM.
+  constructor;
+    unfold returnM, FixM_returnM, bindM, FixM_bindM,
+           FixM_map, FixM_map, proj1_sig;
+    intros; try (apply FixM_eqM_ext; unfold proj1_sig; intros).
+  split; intros.
+  destruct H; destruct H. rewrite H; assumption.
+  exists x; split; [ reflexivity | assumption ].
+  split; intros.
+  destruct H; destruct H. rewrite <- H0; assumption.
+  exists x; split; [ assumption | reflexivity ].
+  split; intros.
+  destruct H; destruct H; destruct H0; destruct H0.
+  exists x1; split; [ | assumption ].
+  exists x0; split; assumption.
+  destruct H; destruct H; destruct H; destruct H.
+  exists x1; split; [ assumption | ].
+  exists x0; split; assumption.
 
-Definition NonTermT (M: Type -> Type) (X:Type) := M (Type01 X).
+  constructor.
+  intros x y H; assumption.
+  intros m1 m2 m3 H1 H2 x pf; apply H2; apply H1; assumption.
 
-Instance NonTermT_returnM `{Monad} : MonadRet (NonTermT M) :=
-  fun A x => returnM (singleton_Type01 x).
-Instance NonTermT_bindM `{Monad} : MonadBind (NonTermT M) :=
-  fun A B m f =>
-    bindM m (fun set => )
+  intros x y e_xy z elem_z; unfold proj1_sig in * |- *.
+  rewrite <- e_xy; assumption.
 
-    fun s => bindM (m s) (fun (sx:S * A) => let (s',x) := sx in f x s').
+  intros m1 m2 leqm f1 f2 leqf x elem_x; unfold proj1_sig in * |- *.
+  destruct elem_x; destruct H. exists x0. split.
+  apply leqm; assumption.
+  apply (leqf x0 x0 eq_refl); assumption.
+Qed.
+
+
+(* The non-termination effects *)
+
+Class MonadFixM (M:Type -> Type) {MonadOrder:MonadOrder M} : Type :=
+  fixM : forall {A B}, ((A -> M B) -> (A -> M B)) -> A -> M B.
+
+Class MonadFix M {MonadRet:MonadRet M} {MonadBind:MonadBind M}
+      {MonadOrder:MonadOrder M} {MonadFixM:MonadFixM M}
+: Prop :=
+  {
+    monad_fix_monad : @Monad M MonadRet MonadBind MonadOrder;
+    monad_fix_fixm :
+      forall A B f x,
+        Proper (respectful (@eq A) (leqM (A:=B)) ==> @eq A ==> leqM (A:=B)) f ->
+        fixM (A:=A) (B:=B) f x == f (fixM f) x
+  }.
+
+
+(* The MonadFix instances for FixM *)
+
+Definition FixM_Bottom {A} : FixM A :=
+  exist (fun P => forall x y, P x /\ P y -> x = y)
+        (fun x => False)
+        (fun x y (H: False /\ False) => match proj1 H with end).
+
+Fixpoint iterate_f {A} n (f: A -> A) :=
+  match n with
+    | 0 => fun x => x
+    | S n' => fun x => f (iterate_f n' f x)
+  end.
+
+Program Instance FixM_fixM : MonadFixM FixM :=
+  fun {A B} f x =>
+    exist _ (fun y =>
+               exists n,
+                 proj1_sig (iterate_f n f (fun _ => FixM_Bottom) x) y
+                 /\ forall n' y',
+                      n' < n ->
+                      ~(proj1_sig (iterate_f n' f (fun _ => FixM_Bottom) x) y')) _.
+Obligation 1.
+destruct (lt_eq_lt_dec H H0) as [ comp | l ]; [ destruct comp | ].
+elimtype False; apply (H2 _ _ l H3).
+rewrite e in H3.
+apply (proj2_sig (iterate_f H0 f (fun _ : A => FixM_Bottom) x)).
+split; assumption.
+elimtype False; apply (H4 _ _ l H1).
+Qed.
+
+(*
+Instance FixM_MonadFix : MonadFix FixM.
+constructor; [ auto with typeclass_instances | ].
+intros. unfold fixM, FixM_fixM.
+apply FixM_eqM_ext; intros; unfold proj1_sig.
 *)
 
 
+(***
+ *** A Better Fixed-Point Monad
+ ***)
+
+(* The idea here is that we only actually care about the first non-None value;
+this way, we don't have any proofs in computations. *)
+Definition FixM2 A := nat -> option A.
+
+(* Get the first value of m at or below n *)
+Fixpoint first_value_below {A} (m:FixM2 A) n : option A :=
+  match n with
+    | 0 => m 0
+    | S n' =>
+      match first_value_below m n' with
+        | Some x => Some x
+        | None => m n
+      end
+  end.
+
+Lemma first_value_below_correct_None {A} m n :
+  @first_value_below A m n = None ->
+  (forall n', n' <= n -> m n' = None).
+  induction n; intros.
+  inversion H0. apply H.
+  unfold first_value_below in H; fold (@first_value_below A) in H.
+  destruct (first_value_below m n); [ discriminate | ].
+  inversion H0.
+  assumption.
+  apply IHn; [ reflexivity | assumption ].
+Qed.
+
+Lemma first_value_below_complete_None {A} m n :
+  (forall n', n' <= n -> m n' = None) ->
+  @first_value_below A m n = None.
+  induction n; intros.
+  apply H; apply le_n.
+  unfold first_value_below; fold (@first_value_below A).
+  rewrite IHn.
+  apply H; apply le_n.
+  intros; apply H; apply le_S; assumption.
+Qed.
+
+Lemma first_value_below_correct_Some {A} m n (x:A) :
+  first_value_below m n = Some x ->
+  exists n', n' <= n /\ m n' = Some x /\ (forall n'', n'' < n' -> m n'' = None).
+  induction n; unfold first_value_below; fold (@first_value_below A); intro H.
+  exists 0; split; [ constructor | split; [ assumption | ] ].
+  intros; inversion H0.
+  case_eq (first_value_below m n); intros; rewrite H0 in * |- *.
+  destruct (IHn H) as [ n' H1 ]; destruct H1; destruct H2.
+  exists n'. split; [ apply le_S; assumption | split; assumption ].
+  exists (S n). split; [ apply le_n | split; [ assumption | ] ].
+  intros. apply (first_value_below_correct_None _ n).
+  assumption.
+  apply le_S_n; assumption.
+Qed.
+
+Lemma first_value_below_complete_Some {A} m n n' (x:A) :
+  n' <= n -> m n' = Some x -> (forall n'', n'' < n' -> m n'' = None) ->
+  first_value_below m n = Some x.
+  intro leq; induction leq; intros.
+  destruct n'.
+  assumption.
+  unfold first_value_below; fold (@first_value_below A).
+  rewrite first_value_below_complete_None; [ assumption | ].
+  intros; apply H0; apply le_n_S; assumption.
+  unfold first_value_below; fold (@first_value_below A).
+  rewrite IHleq; [ reflexivity | assumption | assumption ].
+Qed.
+
+Lemma first_value_below_constant_fun {A} (x:option A) n :
+  first_value_below (fun _ => x) n = x.
+  induction n.
+  reflexivity.
+  unfold first_value_below; fold (@first_value_below A).
+  rewrite IHn; destruct x; reflexivity.
+Qed.
+
+Lemma first_value_below_stable {A} (m:FixM2 A) n n' x :
+  n <= n' -> first_value_below m n = Some x ->
+  first_value_below m n' = Some x.
+  intro l; induction l.
+  unfold first_value_below; fold (@first_value_below A).
+  intro e; rewrite e; reflexivity.
+  unfold first_value_below; fold (@first_value_below A).
+  intro. rewrite (IHl H). reflexivity.
+Qed.
+
+Lemma first_value_below_idempotent {A} (m:FixM2 A) n :
+  first_value_below (fun n' => first_value_below m n') n =
+  first_value_below m n.
+  induction n.
+  reflexivity.
+  unfold first_value_below; repeat (fold (@first_value_below A)).
+  rewrite IHn.
+  destruct (first_value_below m n); reflexivity.
+Qed.
+
+(* True iff the "true" value of m is x *)
+Definition value_is {A} (m:FixM2 A) (x:A) : Prop :=
+  exists n, first_value_below m n = Some x.
+
+Lemma value_is_functional {A} m (x1 x2:A) :
+  value_is m x1 -> value_is m x2 -> x1 = x2.
+  intros vis1 vis2; destruct vis1; destruct vis2.
+  destruct (lt_eq_lt_dec x x0); [ destruct s | ];
+  (assert (Some x1 = Some x2) as helper; [ | injection helper; intros; assumption ]).
+  assert (x <= x0); [ apply le_S_n; apply le_S; assumption | ].
+  rewrite <- H0. rewrite <- (first_value_below_stable _ _ _ _ H1 H). reflexivity.
+  rewrite e in H; rewrite <- H; rewrite <- H0; reflexivity.
+  assert (x0 <= x); [ apply le_S_n; apply le_S; assumption | ].
+  rewrite <- H. rewrite <- (first_value_below_stable _ _ _ _ H1 H0). reflexivity.
+Qed.
+
+Instance FixM2_returnM : MonadRet FixM2 :=
+  fun {A} x => fun n => Some x.
+
+Instance FixM2_bindM : MonadBind FixM2 :=
+  fun {A B} m f =>
+    fun n =>
+      match first_value_below m n with
+        | None => None
+        | Some x => first_value_below (f x) n
+      end.
+
+Instance FixM2_leqM : MonadOrder FixM2 :=
+  fun {A} m1 m2 => forall x, value_is m1 x -> value_is m2 x.
+
+Instance value_is_proper {A} :
+  Proper (eqM (A:=A) ==> @eq A ==> iff) value_is.
+intros m1 m2 em x1 x2 ex. rewrite ex. destruct em as [ em1 em2 ].
+split; intro H.
+apply (em1 x2 H).
+apply (em2 x2 H).
+Qed.
+
+Instance first_value_below_is_proper {A} :
+  Proper (respectful (@eq nat) (@eq (option A)) ==> @eq nat ==> @eq (option A)) first_value_below.
+intros m1 m2 em x1 x2 ex; rewrite ex.
+clear ex; clear x1.
+induction x2; unfold first_value_below; fold (@first_value_below A).
+apply em; reflexivity.
+rewrite IHx2; destruct (first_value_below m2 x2).
+reflexivity.
+apply em; reflexivity.
+Qed.
 
 
+Lemma first_value_below_commute_constant {A B} x (f:A -> nat -> option B) n :
+  first_value_below
+    (fun n =>
+       match first_value_below (fun _ => Some x) n with
+         | Some y => f y n
+         | None => None
+       end) n
+  = first_value_below (f x) n.
+  induction n.
+  reflexivity.
+  unfold first_value_below; fold (@first_value_below A); fold (@first_value_below B).
+  rewrite IHn.
+  rewrite first_value_below_constant_fun.
+  reflexivity.
+Qed.
+
+Lemma first_value_below_bind_None {A B} m f n :
+  first_value_below m n = None ->
+  first_value_below (@FixM2_bindM A B m f) n = None.
+  induction n; intros.
+  unfold first_value_below, FixM2_bindM; rewrite H; reflexivity.
+  unfold first_value_below, FixM2_bindM; fold (@first_value_below B).
+  rewrite H.
+  unfold FixM2_bindM in IHn. rewrite IHn. reflexivity.
+  unfold first_value_below in H; fold (@first_value_below A) in H.
+  destruct (first_value_below m n); [ discriminate | reflexivity ].
+Qed.
+
+Lemma first_value_below_bind_Some {A B} x m f n :
+  first_value_below m n = Some x ->
+  first_value_below (@FixM2_bindM A B m f) n = first_value_below (f x) n.
+  induction n; intros.
+  unfold first_value_below, FixM2_bindM; rewrite H; reflexivity.
+  unfold first_value_below, FixM2_bindM.
+  fold (@first_value_below B).
+  case_eq (first_value_below m n); intros.
+  unfold FixM2_bindM in IHn.
+  rewrite IHn. rewrite H.
+  case_eq (first_value_below (f x) n); intros; [ reflexivity | ].
+  unfold first_value_below; fold (@first_value_below B). rewrite H1. reflexivity.
+  unfold first_value_below in H; fold (@first_value_below A) in H.
+  rewrite H0 in H. rewrite H0. assumption.
+  replace (first_value_below
+             (fun n0 : nat =>
+                match first_value_below m n0 with
+                  | Some x0 => first_value_below (f x0) n0
+                  | None => None
+                end) n) with (@None B).
+  rewrite H. reflexivity.
+  fold (@FixM2_bindM A B m f); symmetry; apply first_value_below_bind_None; assumption.
+Qed.
+
+(* Extensionality law for == on FixM2 *)
+Lemma FixM2_eqM_ext A (m1 m2: FixM2 A) :
+  (forall x, value_is m1 x <-> value_is m2 x) -> m1 == m2.
+  unfold eqM, leqM, FixM2_leqM, value_is; intro e; split; intros; destruct (e x).
+  apply (H0 H).
+  apply (H1 H).
+Qed.
+
+Lemma FixM2_eqM_ext2 A (m1 m2: FixM2 A) :
+  (forall n, first_value_below m1 n = first_value_below m2 n) -> m1 == m2.
+  unfold eqM, leqM, FixM2_leqM, value_is; intro e; split; intros;
+  destruct H as [ n H ]; exists n.
+  rewrite <- e; assumption.
+  rewrite e; assumption.
+Qed.
+
+(*
+Lemma FixM2_eqM_ext2 A (m1 m2: FixM2 A) :
+  (forall x1 x2 n1 n2,
+     first_value_below m1 n1 = Some x1 ->
+     first_value_below m2 n2 = Some x2 -> x1 = x2) -> m1 == m2.
+  unfold eqM, leqM, FixM2_leqM, value_is; intro H; split; intros x H0;
+    destruct H0 as [ n H0 ].
+
+intro e; split; intros; destruct (e x).
+  apply (H0 H).
+  apply (H1 H).
+Qed.
+*)
+
+(* The Monad instance for FixM2 *)
+Instance FixM2_Monad : Monad FixM2.
+  constructor;
+    unfold returnM, FixM2_returnM, bindM; intros;
+  try (apply FixM2_eqM_ext2; intros).
+  unfold FixM2_bindM; rewrite first_value_below_commute_constant;
+  apply first_value_below_idempotent.
+  unfold FixM2_bindM; rewrite <- (first_value_below_idempotent m).
+  apply first_value_below_is_proper; [ | reflexivity ]; intros n1 n2 e; rewrite e.
+  case_eq (first_value_below m n2); intros; [ | reflexivity ].
+  apply first_value_below_constant_fun.
+
+  case_eq (first_value_below m n); intros.
+  rewrite (first_value_below_bind_Some _ _ _ _ H).
+  case_eq (first_value_below (f a) n); intros.
+  assert (first_value_below (FixM2_bindM A B m f) n = Some b).
+  rewrite (first_value_below_bind_Some _ _ _ _ H); assumption.
+  rewrite (first_value_below_bind_Some _ _ _ _ H0).
+  rewrite (first_value_below_bind_Some _ _ _ _ H1).
+  reflexivity.
+  assert (first_value_below (FixM2_bindM A B m f) n = None).
+  rewrite (first_value_below_bind_Some _ _ _ _ H); assumption.
+  rewrite (first_value_below_bind_None _ _ _ H0).
+  rewrite (first_value_below_bind_None _ _ _ H1).
+  reflexivity.
+  rewrite (first_value_below_bind_None _ _ _ H).
+  assert (first_value_below (FixM2_bindM A B m f) n = None).
+  apply (first_value_below_bind_None _ _ _ H).
+  rewrite (first_value_below_bind_None _ _ _ H0).
+  reflexivity.
+
+  constructor.
+  intros m x vis; assumption.
+  intros m1 m2 m3 H1 H2 x vis. apply H2; apply H1; assumption.
+  intros x y e z vis. rewrite <- e; assumption.
+
+  intros m1 m2 leqm f1 f2 leqf y vis.
+  destruct vis as [ n ].
+  assert (exists x, first_value_below m1 n = Some x).
+  case_eq (first_value_below m1 n); intros.
+  exists a; reflexivity.
+  rewrite (first_value_below_bind_None _ _ _ H0) in H; discriminate.
+  destruct H0.
+  destruct (leqm x (ex_intro _ n H0)) as [ n1 ].
+  rewrite (first_value_below_bind_Some _ _ _ _ H0) in H.
+  destruct (leqf x x eq_refl y (ex_intro _ n H)) as [ n2 ].
+  exists (max n1 n2).
+  rewrite (first_value_below_bind_Some x m2 f2).
+  apply (first_value_below_stable _ n2); [ apply Nat.le_max_r | assumption ].
+  apply (first_value_below_stable _ n1); [ apply Nat.le_max_l | assumption ].
+Qed.
